Let’s verify the identity:  

We are given:  
$$
1^3 + 2^3 + 3^3 + \dots + n^3 = \left( \frac{(1+n)n}{2} \right)^2
$$
for \(n\) a positive integer.

---

**Step 1 – Recall known formula for sum of cubes**

The sum of the first \(n\) cubes is:
$$
\sum_{k=1}^{n} k^3 = \frac{n^2(n+1)^2}{4}.
$$
This is a standard identity, often proved by induction or known formulas.

---

**Step 2 – Check RHS of given statement**

The RHS given is:
$$
\left( \frac{(1+n)n}{2} \right)^2 = \frac{n^2 (n+1)^2}{4}.
$$

---

**Step 3 – Compare LHS formula to RHS**

LHS from known formula:

$$
\frac{n^2 (n+1)^2}{4}.
$$

Clearly the RHS is identical:
$$
\frac{n^2 (n+1)^2}{4}.
$$

---

**Step 4 – Verify for a small \(n\)**

For `n=2`:  
LHS: \(1^3 + 2^3 = 1 + 8 = 9\)  
RHS: $$\left(\frac{(1+2) \cdot 2}{2}\right)^2 = \left( \frac{3\cdot 2}{2} \right)^2 = (3)^2 = 9$$ ✓

For `n=3`:  
LHS: \(1+8+27=36\)  
RHS: $$\left( \frac{4\cdot 3}{2} \right)^2 = (6)^2 = 36$$ ✓

---

**Step 5 – Conclusion**

The given equality is true and is the known closed form for the sum of cubes.

$$
\boxed{\text{True}}
$$